external/Goose/github_com/tchajed/marshal.v
@@ -21,13 +21,13 @@ Definition Enc__PutInt: val :=
   rec: "Enc__PutInt" "enc" "x" :=
     let: "off" := ![uint64T] (struct.get Enc.S "off" "enc") in
     UInt64Put (SliceSkip byteT (struct.get Enc.S "b" "enc") "off") "x";;
-    struct.get Enc.S "off" "enc" <-[refT uint64T] ![uint64T] (struct.get Enc.S "off" "enc") + #8.
+    struct.get Enc.S "off" "enc" <-[uint64T] ![uint64T] (struct.get Enc.S "off" "enc") + #8.
 
 Definition Enc__PutInt32: val :=
   rec: "Enc__PutInt32" "enc" "x" :=
     let: "off" := ![uint64T] (struct.get Enc.S "off" "enc") in
     UInt32Put (SliceSkip byteT (struct.get Enc.S "b" "enc") "off") "x";;
-    struct.get Enc.S "off" "enc" <-[refT uint64T] ![uint64T] (struct.get Enc.S "off" "enc") + #4.
+    struct.get Enc.S "off" "enc" <-[uint64T] ![uint64T] (struct.get Enc.S "off" "enc") + #4.
 
 Definition Enc__PutInts: val :=
   rec: "Enc__PutInts" "enc" "xs" :=
@@ -38,7 +38,7 @@ Definition Enc__PutBytes: val :=
   rec: "Enc__PutBytes" "enc" "b" :=
     let: "off" := ![uint64T] (struct.get Enc.S "off" "enc") in
     let: "n" := SliceCopy byteT (SliceSkip byteT (struct.get Enc.S "b" "enc") "off") "b" in
-    struct.get Enc.S "off" "enc" <-[refT uint64T] ![uint64T] (struct.get Enc.S "off" "enc") + "n".
+    struct.get Enc.S "off" "enc" <-[uint64T] ![uint64T] (struct.get Enc.S "off" "enc") + "n".
 
 Definition Enc__Finish: val :=
   rec: "Enc__Finish" "enc" :=
@@ -63,19 +63,19 @@ Definition NewDec: val :=
 Definition Dec__GetInt: val :=
   rec: "Dec__GetInt" "dec" :=
     let: "off" := ![uint64T] (struct.get Dec.S "off" "dec") in
-    struct.get Dec.S "off" "dec" <-[refT uint64T] ![uint64T] (struct.get Dec.S "off" "dec") + #8;;
+    struct.get Dec.S "off" "dec" <-[uint64T] ![uint64T] (struct.get Dec.S "off" "dec") + #8;;
     UInt64Get (SliceSkip byteT (struct.get Dec.S "b" "dec") "off").
 
 Definition Dec__GetInt32: val :=
   rec: "Dec__GetInt32" "dec" :=
     let: "off" := ![uint64T] (struct.get Dec.S "off" "dec") in
-    struct.get Dec.S "off" "dec" <-[refT uint64T] ![uint64T] (struct.get Dec.S "off" "dec") + #4;;
+    struct.get Dec.S "off" "dec" <-[uint64T] ![uint64T] (struct.get Dec.S "off" "dec") + #4;;
     UInt32Get (SliceSkip byteT (struct.get Dec.S "b" "dec") "off").
 
 Definition Dec__GetInts: val :=
   rec: "Dec__GetInts" "dec" "num" :=
     let: "xs" := ref (zero_val (slice.T uint64T)) in
-    let: "i" := ref #0 in
+    let: "i" := ref_to uint64T #0 in
     (for: (λ: <>, ![uint64T] "i" < "num"); (λ: <>, "i" <-[uint64T] ![uint64T] "i" + #1) := λ: <>,
       "xs" <-[slice.T uint64T] SliceAppend uint64T (![slice.T uint64T] "xs") (Dec__GetInt "dec");;
       Continue);;
@@ -85,5 +85,5 @@ Definition Dec__GetBytes: val :=
   rec: "Dec__GetBytes" "dec" "num" :=
     let: "off" := ![uint64T] (struct.get Dec.S "off" "dec") in
     let: "b" := SliceSubslice byteT (struct.get Dec.S "b" "dec") "off" ("off" + "num") in
-    struct.get Dec.S "off" "dec" <-[refT uint64T] ![uint64T] (struct.get Dec.S "off" "dec") + "num";;
+    struct.get Dec.S "off" "dec" <-[uint64T] ![uint64T] (struct.get Dec.S "off" "dec") + "num";;
     "b".
